src/library/constants.cpp
@@ -85,7 +85,7 @@ name const * g_ge = nullptr;
 name const * g_gt = nullptr;
 name const * g_has_add = nullptr;
 name const * g_has_add_add = nullptr;
-name const * g_andthen = nullptr;
+name const * g_has_andthen_andthen = nullptr;
 name const * g_has_bind_and_then = nullptr;
 name const * g_has_bind_bind = nullptr;
 name const * g_has_bind_seq = nullptr;
@@ -472,7 +472,7 @@ void initialize_constants() {
     g_gt = new name{"gt"};
     g_has_add = new name{"has_add"};
     g_has_add_add = new name{"has_add", "add"};
-    g_andthen = new name{"andthen"};
+    g_has_andthen_andthen = new name{"has_andthen", "andthen"};
     g_has_bind_and_then = new name{"has_bind", "and_then"};
     g_has_bind_bind = new name{"has_bind", "bind"};
     g_has_bind_seq = new name{"has_bind", "seq"};
@@ -860,7 +860,7 @@ void finalize_constants() {
     delete g_gt;
     delete g_has_add;
     delete g_has_add_add;
-    delete g_andthen;
+    delete g_has_andthen_andthen;
     delete g_has_bind_and_then;
     delete g_has_bind_bind;
     delete g_has_bind_seq;
@@ -1247,7 +1247,7 @@ name const & get_ge_name() { return *g_ge; }
 name const & get_gt_name() { return *g_gt; }
 name const & get_has_add_name() { return *g_has_add; }
 name const & get_has_add_add_name() { return *g_has_add_add; }
-name const & get_andthen_name() { return *g_andthen; }
+name const & get_has_andthen_andthen_name() { return *g_has_andthen_andthen; }
 name const & get_has_bind_and_then_name() { return *g_has_bind_and_then; }
 name const & get_has_bind_bind_name() { return *g_has_bind_bind; }
 name const & get_has_bind_seq_name() { return *g_has_bind_seq; }
