tests/lean/out_param_proj.lean
@@ -1,0 +1,6 @@
+universes u v
+class module (α : out_param $ Type u) (β : Type v) [out_param $ ring α] extends add_comm_group β :=
+(foo : β → nat)
+
+-- both α and `ring α` should be implicit (_not_ instance implicit)
+#print module.to_add_comm_group
