tests/lean/run/check_constants.lean
@@ -85,7 +85,7 @@ run_cmd script_check_id `ge
 run_cmd script_check_id `gt
 run_cmd script_check_id `has_add
 run_cmd script_check_id `has_add.add
-run_cmd script_check_id `andthen
+run_cmd script_check_id `has_andthen.andthen
 run_cmd script_check_id `has_bind.and_then
 run_cmd script_check_id `has_bind.bind
 run_cmd script_check_id `has_bind.seq
